<?xml version="1.0" encoding="utf-8"?>
<rdf:RDF xmlns:ldp="http://www.w3.org/ns/ldp#" xmlns:rdfs="http://www.w3.org/2000/01/rdf-schema#" xmlns:owl="http://www.w3.org/2002/07/owl#" xmlns:rdf="http://www.w3.org/1999/02/22-rdf-syntax-ns#" xmlns:dcterms="http://purl.org/dc/terms/" xmlns:vs="http://www.w3.org/2003/06/sw-vocab-status/ns#">
	<owl:Ontology rdf:about="http://www.w3.org/ns/ldp#">
		<dcterms:description>All vocabulary URIs defined in the Linked Data Platform (LDP) namespace.</dcterms:description>
		<dcterms:title>The W3C Linked Data Platform (LDP) Vocabulary</dcterms:title>
		<rdfs:label>W3C Linked Data Platform (LDP)</rdfs:label>
		<rdfs:comment>This ontology provides an informal representation of the concepts and terms as defined in the LDP specification. Consult the LDP specification for normative reference.</rdfs:comment>
		<rdfs:seeAlso rdf:resource="http://www.w3.org/2012/ldp"/>
		<rdfs:seeAlso rdf:resource="http://www.w3.org/TR/ldp-ucr/"/>
		<rdfs:seeAlso rdf:resource="http://www.w3.org/TR/ldp/"/>
		<rdfs:seeAlso rdf:resource="http://www.w3.org/2011/09/LinkedData/"/>
	</owl:Ontology>

	<rdfs:Class rdf:about="http://www.w3.org/ns/ldp#Resource">
		<rdfs:comment>A HTTP-addressable resource with a linked data representation.</rdfs:comment>
		<vs:term_status>unstable</vs:term_status>
		<rdfs:isDefinedBy rdf:resource="http://www.w3.org/ns/ldp#"/>
		<rdfs:label>Resource</rdfs:label>
	</rdfs:Class>

	<rdfs:Class rdf:about="http://www.w3.org/ns/ldp#Container">
		<rdfs:subClassOf rdf:resource="http://www.w3.org/ns/ldp#Resource"/>
		<rdfs:comment>
			A Linked Data Platform Resource (LDPR) that also conforms to
			additional patterns and conventions for managing membership.
			Readers should refer to the specification defining this ontology for the list of
			behaviors associated with it.
		</rdfs:comment>
		<vs:term_status>unstable</vs:term_status>
		<rdfs:isDefinedBy rdf:resource="http://www.w3.org/ns/ldp#"/>
		<rdfs:label>Container</rdfs:label>
	</rdfs:Class>

	<rdfs:Class rdf:about="http://www.w3.org/ns/ldp#AggregateContainer">
		<rdfs:subClassOf rdf:resource="http://www.w3.org/ns/ldp#Container"/>
		<rdfs:comment>
			A Linked Data Platform Container (LDPC) that also conforms to
			additional patterns and conventions for managing members.  It is distinguished from
			CompositeContainer by the following behaviors:
			(1) Clients cannot assume that an AggregateContainer, when deleted, deletes its members.

			While every attempt is made to be complete in this list, readers should also refer
			to the specification defining this ontology.
		</rdfs:comment>
		<vs:term_status>unstable</vs:term_status>
		<rdfs:isDefinedBy rdf:resource="http://www.w3.org/ns/ldp#"/>
		<rdfs:label>AggregateContainer</rdfs:label>
	</rdfs:Class>

	<rdfs:Class rdf:about="http://www.w3.org/ns/ldp#CompositeContainer">
		<rdfs:subClassOf rdf:resource="http://www.w3.org/ns/ldp#Container"/>
		<rdfs:comment>
			A Linked Data Platform Container (LDPC) that also conforms to
			additional patterns and conventions for managing members.  It is distinguished from
			AggregateContainer by the following behaviors:
			(1) An CompositeContainer, when deleted, must delete all its members.

			While every attempt is made to be complete in this list, readers should also
			refer to the specification defining this ontology.
		</rdfs:comment>
		<vs:term_status>unstable</vs:term_status>
		<rdfs:isDefinedBy rdf:resource="http://www.w3.org/ns/ldp#"/>
		<rdfs:label>CompositeContainer</rdfs:label>
	</rdfs:Class>

	<rdf:Property rdf:about="http://www.w3.org/ns/ldp#containerSortPredicates">
		<rdfs:comment>List of predicates that indicate the ascending order of the members in a page.</rdfs:comment>
		<vs:term_status>unstable</vs:term_status>
		<rdfs:domain rdf:resource="http://www.w3.org/ns/ldp#Page"/>
		<rdfs:isDefinedBy rdf:resource="http://www.w3.org/ns/ldp#"/>
		<rdfs:label>containerSortPredicates</rdfs:label>
		<rdfs:range rdf:resource="http://www.w3.org/1999/02/22-rdf-syntax-ns#List"/>
	</rdf:Property>

	<rdf:Property rdf:about="http://www.w3.org/ns/ldp#membershipPredicate">
		<rdfs:comment>Indicates which predicate of the container should be used to determine the membership.</rdfs:comment>
		<vs:term_status>unstable</vs:term_status>
		<rdfs:domain rdf:resource="http://www.w3.org/ns/ldp#Container"/>
		<rdfs:isDefinedBy rdf:resource="http://www.w3.org/ns/ldp#"/>
		<rdfs:label>membershipPredicate</rdfs:label>
		<rdfs:range rdf:resource="http://www.w3.org/1999/02/22-rdf-syntax-ns#Property"/>
	</rdf:Property>

	<rdf:Property rdf:about="http://www.w3.org/ns/ldp#membershipSubject">
		<rdfs:comment>Indicates which resource is the subject for the members of the container.</rdfs:comment>
		<vs:term_status>unstable</vs:term_status>
		<rdfs:domain rdf:resource="http://www.w3.org/ns/ldp#Container"/>
		<rdfs:isDefinedBy rdf:resource="http://www.w3.org/ns/ldp#"/>
		<rdfs:label>membershipSubject</rdfs:label>
		<rdfs:range rdf:resource="http://www.w3.org/1999/02/22-rdf-syntax-ns#Property"/>
	</rdf:Property>

	<rdf:Property rdf:about="http://www.w3.org/ns/ldp#nextPage">
		<rdfs:comment>From a known page, how to indicate the next or last page as rdf:nil.</rdfs:comment>
		<vs:term_status>unstable</vs:term_status>
		<rdfs:domain rdf:resource="http://www.w3.org/ns/ldp#Page"/>
		<rdfs:isDefinedBy rdf:resource="http://www.w3.org/ns/ldp#"/>
		<rdfs:label>nextPage</rdfs:label>
		<rdfs:range rdf:resource="http://www.w3.org/2000/01/rdf-schema#Resource"/>
	</rdf:Property>

	<rdfs:Class rdf:about="http://www.w3.org/ns/ldp#Page">
		<rdfs:comment>A resource that represents a limited set of members of a LDP Container.</rdfs:comment>
		<vs:term_status>unstable</vs:term_status>
		<rdfs:isDefinedBy rdf:resource="http://www.w3.org/ns/ldp#"/>
		<rdfs:label>Page</rdfs:label>
	</rdfs:Class>

	<rdf:Property rdf:about="http://www.w3.org/ns/ldp#pageOf">
		<rdfs:comment>Associated a page with its container.</rdfs:comment>
		<vs:term_status>unstable</vs:term_status>
		<rdfs:domain rdf:resource="http://www.w3.org/ns/ldp#Page"/>
		<rdfs:isDefinedBy rdf:resource="http://www.w3.org/ns/ldp#"/>
		<rdfs:label>pageOf</rdfs:label>
		<rdfs:range rdf:resource="http://www.w3.org/ns/ldp#Container"/>
	</rdf:Property>
</rdf:RDF>

